Changed refinement of ordinal set to seq of nat

refinements/ordseq.v
@@ -18,17 +18,17 @@ Section ordseq_op.
 (* Variable A : eqType. *)
 Variable N : Type.
 
-Definition ordseq {m} := seq 'I_m.
+Definition ordseq := fun (_ : nat) => seq nat.
 
 Context `{zero_of N, one_of N, add_of N, eq_of N, leq_of N, lt_of N, spec_of N nat}.
 
-Global Instance ordseq0 {m} : zero_of (@ordseq m) := [::].
-Global Instance eq_ordseq {m} : eq_of (@ordseq m) := @eqseq (ordinal_eqType m).
+Global Instance ordseq0 {m} : zero_of (ordseq m) := [::].
+Global Instance eq_ordseq {m} : eq_of (ordseq m) := @eqseq nat_eqType.
 
-Fixpoint ordseq_sublist {m} (p q : ordseq) : bool :=
+Fixpoint ordseq_sublist {m} (p q : ordseq m) : bool :=
   (* mem_aux : returns true/false, plus the remaining list after the match
                in case the element has indeed been found *)
-  let fix mem_aux (x : 'I_m) (p' : ordseq) : bool * ordseq := match p' with
+  let fix mem_aux x (p' : ordseq m) : bool * (ordseq m) := match p' with
   | [::] => (false, [::])
   | h :: t =>
       (* If element is found, return true and the rest of the other set *)
@@ -45,10 +45,10 @@ Fixpoint ordseq_sublist {m} (p q : ordseq) : bool :=
   end.
 
 (* Difference of two ordseqs *)
-Definition ordseq_sub {m} : sub_of (@ordseq m) :=
-  let fix aux (a : ordseq) : ordseq -> ordseq := match a with
+Definition ordseq_sub {m} : sub_of (ordseq m) :=
+  let fix aux (a : ordseq m) : ordseq _ -> ordseq _ := match a with
   | [::] => fun _ => [::]
-  | h :: t => (fix aux_comp (b : ordseq) : ordseq :=
+  | h :: t => (fix aux_comp (b : ordseq _) : ordseq _ :=
       match b with
       | [::] => a
       | h' :: t' =>
@@ -62,24 +62,26 @@ Definition ordseq_sub {m} : sub_of (@ordseq m) :=
 Definition ordcmp {m} := fun (x y : 'I_m) => ((nat_of_ord x) <= (nat_of_ord y))%N.
 
 (* Union of two ordseqs *)
-Definition ordseq_add {m} `{spec_of N 'I_m} : add_of (@ordseq m) :=
-  fun a b => merge ordcmp a (ordseq_sub a b).
+Definition ordseq_add {m} `{spec_of N 'I_m} : add_of (ordseq m) :=
+  fun a b => merge leqn a (ordseq_sub a b).
 
 (** Returning if an element is a member of a set *)
-Fixpoint ordseq_mem {m} (x : 'I_m) (p : ordseq) : bool := match p with
+Fixpoint ordseq_mem {m} x (p : ordseq m) : bool := match p with
   | [::] => false
-  | h :: t => (h == x) || ordseq_mem x t
+  | h :: t => (h == x) || @ordseq_mem m x t
   end.
 
-Global Instance implem_ordseq m : implem_of {set 'I_m} ordseq :=
-  fun s => [seq i | i <- enum s].
+Global Instance implem_ordseq {m} : implem_of {set 'I_m} (ordseq m) :=
+  fun s => [seq (nat_of_ord i) | i <- enum s].
 
-Global Instance spec_ordseq {m} `{spec_of N 'I_m} :
+(* TODO: We need a spec_of nat 'I_m somehow! *)
+Global Instance spec_ordseq {m} `{H : spec_of nat 'I_m} :
   spec_of (@ordseq m) {set 'I_m} := fun s =>
-  [set i | i \in s].
+  let sMapped := map (@spec _ _ H) s in
+  [set i | i \in sMapped].
 
 (** Size of a set *)
-Global Instance size_seqset {m} : size_of (@ordseq m) N :=
+Global Instance size_seqset {m} : size_of (ordseq m) N :=
   let fix aux cnt p := match p with
   | [::] => cnt
   | _ :: t => aux (cnt + 1) t
@@ -90,15 +92,23 @@ Local Open Scope rel_scope.
 
 (* In the spirit of Rseqmx...*)
 CoInductive Rordseq {m1 m2} (rm : nat_R m1 m2) :
-  {set 'I_m1} -> @ordseq m2 -> Type := Rordseq_spec (I : {set 'I_m1}) (J : ordseq) of
-  (forall j, j \in J -> ((nat_of_ord j) < m1)%N) &
-  (uniq J) & (sorted ordcmp J) : Rordseq rm I J.
+  {set 'I_m1} -> @ordseq m2 -> Type := Rordseq_spec (I : {set 'I_m1}) (J : ordseq m2) of
+  (forall j, j \in J -> (j < m1)%N) &
+  (uniq J) & (sorted leqn J) : Rordseq rm I J.
 
 Instance Rordseq_add {m1 m2} (rm : nat_R m1 m2)
 (I : 'I_m1) (J : (@ordseq m2)) `{Hm: spec_of N 'I_m2} :
   refines (Rordseq rm ==> Rordseq rm ==> Rordseq rm)
   (@setU (ordinal_finType m1)) (@ordseq_add m2 Hm).
 Proof.
-  rewrite refinesE; constructor.
+  rewrite refinesE => I' J' Ho Ialt Jalt Ho'; constructor.
+  - admit.
+  - rewrite /ordseq_add merge_uniq cat_uniq. admit.
+  - rewrite /ordseq_add merge_sorted //=.
+    + rewrite /total => x1 y1.
+      case/boolP: (leqn x1 y1) => [// |].
+      by rewrite orFb -ltnNge ltn_neqAle => /andP[_ ?] //.
+    + by case: Ho.
+    + admit.
   (** TODO: Do this! **)
 Admitted.
